backend/CleanupLabelstyping.v
@@ -22,7 +22,7 @@ Require Import CleanupLabels.
 Require Import LTLintyping.
 
 Section WITHEF.
-Context `{Hef: ExternalFunctions}.
+Context `{Hsc: SyntaxConfiguration}.
 
 Lemma in_remove_unused_labels:
   forall bto i c, In i (remove_unused_labels bto c) -> In i c.
