cfrontend/Initializers.v
@@ -26,7 +26,7 @@ Require Import Csyntax.
 Open Scope error_monad_scope.
 
 Section WITHMEM.
-Context `{Hef: ExternalFunctions}.
+Context `{Hsc: SyntaxConfiguration}.
 Context `{Hmem: Mem.MemoryModel}.
 
 (** * Evaluation of compile-time constant expressions *)
